map wip

Matroid/Constructions/DirectSum.lean
@@ -8,7 +8,7 @@ variable {α β ι : Type*}
 
 -- a little API for mathlib.
 
-/-- If `s` and `t` are disjoint sets in `α`, there is a natural injection from `s ⊕ t` to `α`. -/
+/-- For disjoint `s t : Set α`, the natural injection from `↑s ⊕ ↑t` to `α`. -/
 @[simps] def Disjoint.sumSubtypeEmbedding {s t : Set α} (h : Disjoint s t) : s ⊕ t ↪ α where
   toFun := Sum.elim Subtype.val Subtype.val
   inj' := by
@@ -30,7 +30,30 @@ variable {α β ι : Type*}
     range h.sumSubtypeEmbedding = s ∪ t := by
   ext; simp
 
+/-- For an indexed family `s` of disjoint sets in `α`, the natural injection from the
+sigma-type `(i : ι) × ↑(s i)` to `α`. -/
+@[simps] def Set.PairwiseDisjoint.sigmaSubtypeEmbedding {s : ι → Set α}
+    (h : PairwiseDisjoint univ s) : ((i : ι) × (s i)) ↪ α where
+      toFun := fun ⟨i, x⟩ ↦ x.1
+      inj' := by
+        rintro ⟨i,x⟩ ⟨j,y⟩ (hxy : x.1 = y.1)
+        obtain rfl : i = j := Set.PairwiseDisjoint.elim h (mem_univ i) (mem_univ j)
+          (not_disjoint_iff.2 ⟨x.1,x.2, by rw [hxy]; exact y.2⟩)
+        rw [Subtype.val_inj] at hxy
+        rw [hxy]
+
+@[simp] theorem Set.PairwiseDisjoint.sigmaSubtypeEmbedding_preimage {s : ι → Set α}
+    (h : PairwiseDisjoint univ s) (i : ι) (r : Set α) :
+    Sigma.mk i ⁻¹' (h.sigmaSubtypeEmbedding ⁻¹' r) = r ∩ (s i) := by
+  ext; simp
+
+@[simp] theorem Set.PairwiseDisjoint.sigmaSubtypeEmbedding_range {s : ι → Set α}
+    (h : PairwiseDisjoint univ s) : Set.range h.sigmaSubtypeEmbedding = ⋃ i : ι, s i := by
+  ext; simp
+
 namespace Matroid
+
+section Sigma
 
 /-- We prove that the direct sum of an indexed collection of matroids is a matroid
   by constructing an `IndepMatroid`.
@@ -46,8 +69,8 @@ private def sigmaIndepMatroid {α : ι → Type*} (M : (i : ι) → Matroid (α 
       indep_maximal := sorry
       subset_ground := sorry
 
-/-- An indexed collection of matroids on arbitrary types determines a
-  'direct sum' matroid on the sigma-type. -/
+/-- An indexed collection of matroids on arbitrary types determines a 'direct sum' matroid
+on the sigma-type. -/
 def sigma {α : ι → Type*} (M : (i : ι) → Matroid (α i)) : Matroid ((i : ι) × α i) :=
   (sigmaIndepMatroid M).matroid
 
@@ -58,6 +81,23 @@ def sigma {α : ι → Type*} (M : (i : ι) → Matroid (α i)) : Matroid ((i : 
 @[simp] theorem sigma_ground_eq {α : ι → Type*} {M : (i : ι) → Matroid (α i)} :
   (sigma M).E = ⋃ (i : ι), (Sigma.mk i '' (M i).E) := rfl
 
+/-- The direct sum of an indexed collection of matroids on `α` with disjoint ground sets. -/
+def sigma' (M : ι → Matroid α) (h : PairwiseDisjoint univ (fun i ↦ (M i).E)) : Matroid α :=
+  (sigma (fun i ↦ (M i).restrictSubtype (M i).E)).mapEmbedding h.sigmaSubtypeEmbedding
+
+@[simp] theorem sigma'_ground_eq {M : ι → Matroid α} (h : PairwiseDisjoint univ (fun i ↦ (M i).E)) :
+    (sigma' M h).E = ⋃ i : ι, (M i).E := by
+  ext; simp [sigma', mapEmbedding, restrictSubtype]
+
+@[simp] theorem sigma'_indep_iff {M : ι → Matroid α} {h : PairwiseDisjoint univ (fun i ↦ (M i).E)}
+    {I : Set α} :
+    (sigma' M h).Indep I ↔ (∀ i, (M i).Indep (I ∩ (M i).E)) ∧ I ⊆ ⋃ i : ι, (M i).E := by
+  simp [sigma', h.sigmaSubtypeEmbedding_preimage]
+
+end Sigma
+
+section Sum
+
 /-- The direct sum of two matroids. Defined in terms of `Matroid.sigma` and
 ``Equiv.sumEquivSigmaBool`, which requires handling some universe issues with `ULift`. -/
 def directSum {α : Type u} {β : Type v} (M : Matroid α) (N : Matroid β) : Matroid (α ⊕ β) :=
@@ -67,7 +107,7 @@ def directSum {α : Type u} {β : Type v} (M : Matroid α) (N : Matroid β) : Ma
   S'.mapEquiv (Equiv.sumCongr Equiv.ulift Equiv.ulift)
 
 /-- Because of this simp lemma, the ugly universe stuff in the implementation of `directSum`
-  doesn't matter. -/
+doesn't matter. -/
 @[simp] theorem directSum_indep_iff {M : Matroid α} {N : Matroid β} {I : Set (α ⊕ β)} :
     (M.directSum N).Indep I ↔ M.Indep (.inl ⁻¹' I) ∧ N.Indep (.inr ⁻¹' I) := by
   simp only [directSum, mapEquiv_indep_iff, Equiv.sumCongr_symm, Equiv.sumCongr_apply,
@@ -78,7 +118,7 @@ def directSum {α : Type u} {β : Type v} (M : Matroid α) (N : Matroid β) : Ma
     (M.directSum N).E = (.inl '' M.E) ∪ (.inr '' N.E) := by
   ext; simp [directSum, mapEquiv, mapEmbedding, Equiv.ulift, Equiv.sumEquivSigmaBool]
 
-/-- The direct sum of two `Matroid α` with disjoint ground sets, defined as a `Matroid α`.
+/-- The direct sum of two matroids on `α` with disjoint ground sets, as a `Matroid α`.
 Implemented by mapping a matroid on `M.E ⊕ N.E` into `α`.  -/
 def directSum' (M N : Matroid α) (h : Disjoint M.E N.E) : Matroid α :=
   ((M.restrictSubtype M.E).directSum (N.restrictSubtype N.E)).mapEmbedding h.sumSubtypeEmbedding
@@ -91,7 +131,13 @@ def directSum' (M N : Matroid α) (h : Disjoint M.E N.E) : Matroid α :=
     (M.directSum' N h).Indep I ↔ M.Indep (I ∩ M.E) ∧ N.Indep (I ∩ N.E) ∧ I ⊆ M.E ∪ N.E := by
   simp [directSum', and_assoc]
 
--- TODO - direct sum of arbitrary indexed collections of matroids on the same type
--- with `PairwiseDisjoint` ground sets.
+theorem Indep.eq_union_image_of_directSum {M N : Matroid α} {h : Disjoint M.E N.E}
+    {I : Set α} (hI : (directSum' M N h).Indep I) :
+    ∃ IM IN, M.Indep IM ∧ N.Indep IN ∧ Disjoint IM IN ∧ I = IM ∪ IN := by
+  rw [directSum'_indep_iff] at hI
+  refine ⟨I ∩ M.E, I ∩ N.E, hI.1, hI.2.1, h.mono inf_le_right inf_le_right, ?_⟩
+  rw [← inter_union_distrib_left, inter_eq_self_of_subset_left hI.2.2]
+
+end Sum
 
 end Matroid
