Matroid/ForMathlib/Logic_Embedding_Set.lean
@@ -1,0 +1,81 @@
+import Mathlib.Logic.Embedding.Set
+import Mathlib.Tactic
+
+open Set Function
+
+section embeddingInsert
+
+variable {α β γ : Type*} {a : α} {b : β} {s : Set α} {f : s ↪ β}
+
+
+@[simp] theorem range_embeddingOfSubset {s t : Set α} (hst : s ⊆ t) :
+    range (embeddingOfSubset s t hst) = {x | x.1 ∈ s} := by
+  ext ⟨x,hx⟩; simp [embeddingOfSubset]
+
+theorem embeddingOfSubset_apply {s t : Set α} (hst : s ⊆ t) (x : s) :
+    embeddingOfSubset s t hst x = ⟨x.1, hst x.2⟩ := rfl
+
+-- this should be elsewhere.
+theorem Embedding.range_trans {f : α ↪ β} {g : β ↪ γ} : range (f.trans g) = g '' (range f) :=
+  range_comp g f
+
+-- this is an `apply_coe` lemma in mathlib that should be renamed.
+-- @[simp] theorem embeddingOfSubset_apply_val {s t : Set α} (hst : s ⊆ t) (x : s) :
+--     (embeddingOfSubset s t hst x).1 = x.1 := rfl
+
+/-- An embedding defined on a coerced set can be extended to an embedding on an insertion. -/
+noncomputable def Subtype.embeddingInsert (f : s ↪ β) (ha : a ∉ s) (hb : b ∉ range f) :
+    ↑(insert a s) ↪ β where
+  toFun := Function.extend (embeddingOfSubset _ _ (subset_insert a s)) f (fun _ ↦ b)
+  inj' := by
+    have hinj := (embeddingOfSubset _ _ (subset_insert a s)).injective
+    have aux : ∀ (x : ↑(insert a s)),
+        x = ⟨a, mem_insert _ _⟩ ∨ ∃ (x₀ : s), x = embeddingOfSubset _ _ (subset_insert a s) x₀ := by
+      rintro ⟨x, (rfl | hx)⟩; exact .inl rfl; exact .inr ⟨⟨x,hx⟩, rfl⟩
+    rintro x y hxy
+    obtain (rfl | ⟨x₀,rfl⟩) := aux x
+    · rw [extend_apply' _ _ _ (by simpa [embeddingOfSubset])] at hxy
+      obtain (rfl | ⟨y₀,rfl⟩) := aux y
+      · rfl
+      rw [hinj.extend_apply] at hxy
+      simp [hxy] at hb
+    rw [hinj.extend_apply] at hxy
+    obtain (rfl | ⟨y₀,rfl⟩) := aux y
+    · rw [extend_apply' _ _ _ (by simpa [embeddingOfSubset])] at hxy
+      simp [hxy.symm] at hb
+    rw [hinj.extend_apply, f.apply_eq_iff_eq] at hxy
+    rw [hxy]
+
+theorem Subtype.embeddingInsert_apply_mem (f : s ↪ β) (ha : a ∉ s) (hb : b ∉ range f)
+    {x : ↑(insert a s)} (hx : x.1 ∈ s) : (Subtype.embeddingInsert f ha hb) x = f ⟨x,hx⟩ := by
+  nth_rw 1 [show x = embeddingOfSubset _ _ (subset_insert a s) ⟨x,hx⟩ from rfl]
+  simp [embeddingInsert, (embeddingOfSubset _ _ (subset_insert a s)).injective.extend_apply]
+
+theorem Subtype.embeddingInsert_apply (f : s ↪ β) (ha : a ∉ s) (hb : b ∉ range f) :
+    (Subtype.embeddingInsert f ha hb) ⟨a, mem_insert _ _⟩ = b := by
+  simp only [embeddingInsert, Embedding.coeFn_mk]
+  rw [extend_apply' _ _ _ (by simpa [embeddingOfSubset])]
+
+theorem Subtype.embeddingInsert_apply' (f : s ↪ β) (ha : a ∉ s) (hb : b ∉ range f)
+    {x : ↑(insert a s)} (hx : x.1 ∉ s) : (Subtype.embeddingInsert f ha hb) x = b := by
+  obtain ⟨x, (rfl | h)⟩ := x
+  · rw [Subtype.embeddingInsert_apply]
+  exact (hx h).elim
+
+theorem Subtype.embeddingInsert_apply_eq_ite (f : s ↪ β) (ha : a ∉ s) (hb : b ∉ range f)
+    {x : ↑(insert a s)} [DecidablePred (· ∈ s)] :
+    (Subtype.embeddingInsert f ha hb) x = if hx : x.1 ∈ s then f ⟨x,hx⟩ else b := by
+  split_ifs with h
+  · rw [embeddingInsert_apply_mem]
+  rwa [embeddingInsert_apply']
+
+@[simp] theorem Subtype.range_embeddingInsert (f : s ↪ β) (ha : a ∉ s) (hb : b ∉ range f) :
+    range (Subtype.embeddingInsert f ha hb) = insert b (range f) := by
+  simp only [embeddingInsert, Embedding.coeFn_mk]
+  rw [range_extend (embeddingOfSubset _ _ (subset_insert a s)).injective, range_embeddingOfSubset]
+  simp_rw [← union_singleton]
+  convert rfl
+  ext x
+  simp [ha, eq_comm (a := x)]
+
+end embeddingInsert
